floyd/SeparationLogicAsLogicSoundness.v
@@ -25,7 +25,6 @@ Require Import VST.veric.semax_switch.
 Require Import VST.veric.semax_prog.
 Require Import VST.veric.semax_ext.
 Require Import VST.veric.SeparationLogic.
-Require Import VST.veric.expr_rel.
 Require Import VST.floyd.SeparationLogicFacts.
 Require Import VST.floyd.SeparationLogicAsLogic.
 Require Import VST.veric.SeparationLogicSoundness.
